\documentclass{article}
\usepackage{fancyhdr}

\begin{document}

\pagenumbering{gobble}

\pagestyle{fancy}
\fancyhead[L]{William Pol 400450462}
\fancyhead[R]{2DM3}


1.1
\[ \frac{x = x + 2}{4 * x + y = \mathord{?}} \]

\[ \frac{x = x + 2}{4 * x + y = 4 * (x + 2) + y} \]

\[ E = 4 * z + y \]

\vspace{10mm}
1.2
\[ \frac{2 * y + 1 = 5}{x + (2 * y + 1) * w = \mathord{?}} \]

\[ \frac{2 * y + 1 = 5}{x + (2 * y + 1) * w = x + 5 * w} \]

\[ E = x + z * w \]

\vspace{10mm}
1.3
\[ \frac{x + 1 = y}{3 * (x + 1) + 3 * x + 1 = \mathord{?}} \]

\[ \frac{x + 1 = y}{3 * (x + 1) + 3 * x + 1 = 3 * y + 3 * x + 1} \]

\[ E = 3 * z + 3 * x + 1 \]

\vspace{10mm}
1.4
\[ \frac{x = y}{x + x = \mathord{?}} \]

\[ 
    \frac{x = y}{x + x = x + y} \hspace{10mm} 
    \frac{x = y}{x + x = y + x} \hspace{10mm} 
    \frac{x = y}{x + x = y + y}
\]

\[
    E = x + z \hspace{16mm}
    E = z + x \hspace{16mm}
    E = z + z
\]

\newpage

2.1
\begin{center}
    \begin{tabular}{c c|c||c}
         $p$ & $q$ & \( p \land q \) & \( (p \land q) \Longrightarrow p\) \\
         \hline
         False & False & False & True \\
         False & True & False & True \\
         True & False & False & True \\
         True & True & True & True \\
    \end{tabular}
    This expression is a tautology.
\end{center}

2.2
\begin{center}
    \begin{tabular}{c c|c|c||c}
         $p$ & $q$ & \( \neg p \) & \( p \Longrightarrow q \) & \( \neg p \Longrightarrow (p \Longrightarrow q) \) \\
         \hline
         False & False & True & True & True \\
         False & True & True & True & True \\
         True & False & False & False & True \\
         True & True & False & True & True \\
    \end{tabular}
\end{center}
\begin{center} This expression is a tautology. \end{center}

2.3
\begin{center}
    \begin{tabular}{c c|c||c}
         $p$ & $q$ & \( p \vee q \) & \( p \Longrightarrow (p \vee q) \) \\
         \hline
         False & False & False & True \\
         False & True & True & True \\
         True & False & True & True \\
         True & True & True & True \\
    \end{tabular}
    This expression is a tautology.
\end{center}

\vspace{10mm}
3
\begin{center}
    \begin{tabular}{c c|c||c c|c}
         $p$ & $q$ & \( \neg (p \land q) \) & $\neg p$ & $\neg q$ & \( \neg p \vee \neg q \) \\
         \hline
         False & False & True & True & True & True \\
         False & True & True & True & False & True \\
         True & False & True & False & True & True \\
         True & True & False & False & False & False \\
    \end{tabular}
\end{center}
\begin{center} These expressions are equivalent. \end{center}

\newpage

4a) The election has not been decided. \\

b) The election has not been decided, but the votes have been counted. \\

c) If the votes have not been counted, then the election has not been decided. \\

d) The election will be decided if and only if the votes have been counted. \\

e) Either the election is decided or the votes have been counted or both. \\

f) If the votes have been counted, then the election has been decided. \\

g) The election is not decided only if the votes have not been counted. \\

h) Either the votes have not been counted or the votes have been counted, but the election has not been decided. \\

\vspace{10mm}
5a) \( p \land q \) \\

b) \( p \land \neg q \) \\

c) \( \neg p \land \neg q \) \\

d) \( p \vee q \) \\

e) \( p \Longrightarrow q \) \\

f) \( p \not\equiv q \) \\

g) \( p \equiv q \) \\

\newpage

6a) If John Do has the flu, then he will miss the final examination. \\

b) John Do does the final examination if and only if he misses the course. \\

c) If John Do misses the final examination, he will take the course. \\

d) John Do either has the flu, misses the final examination, misses the course or all three. \\

e) For John Do to take the course, it is sufficient for him to either have the flu or miss the final examination. \\

f) Either John Do has the flu and misses the final examination, or he does the final examination and misses the course. \\

\vspace{10mm}
7
\begin{center}
    \begin{tabular}{c|c||c}
        $p$ & \( p \vee \textrm{False} \) & \( p \vee \textrm{False} \equiv p \) \\
        \hline
        False & False & True \\
        True & True & True \\
    \end{tabular}
    The expression is valid.
\end{center}

\end{document}